For the moment, don't use datatype methods in IndirectionTableImpl

Impl/IndirectionTableImpl.i.dfy
@@ -46,7 +46,7 @@ module IndirectionTableImpl {
   // table. We could use a null indirection table instead, it's just slightly more
   // annoying to do that because we'd need additional invariants.
   function method IndirectionTableEmptyConstructor() : linear indirectionTable
-  ensures IndirectionTableEmptyConstructor().Inv()
+  ensures It.Inv(IndirectionTableEmptyConstructor())
   {
     linear var t0 := LinearMutableMap.Constructor<IndirectionTableModel.Entry>(128);
     // This is not important, but needed to satisfy the Inv:
@@ -60,8 +60,8 @@ module IndirectionTableImpl {
   }
 
   function method IndirectionTableRootOnlyConstructor(loc: Location) : linear indirectionTable
-  ensures IndirectionTableRootOnlyConstructor(loc).Inv()
-  ensures IndirectionTableRootOnlyConstructor(loc).I() == IndirectionTableModel.ConstructorRootOnly(loc)
+  ensures It.Inv(IndirectionTableRootOnlyConstructor(loc))
+  ensures It.I(IndirectionTableRootOnlyConstructor(loc)) == IndirectionTableModel.ConstructorRootOnly(loc)
   {
     linear var t0 := LinearMutableMap.Constructor<IndirectionTableModel.Entry>(128);
     linear var t1 := LinearMutableMap.Insert(t0, BT.G.Root(), IndirectionTableModel.Entry(Some(loc), [], 1));
@@ -74,7 +74,7 @@ module IndirectionTableImpl {
       /* refUpperBound = */ BT.G.Root(),
       None);
 
-    assert r.I() == IndirectionTableModel.ConstructorRootOnly(loc); // observe (surprisingly)
+    assert It.I(r) == IndirectionTableModel.ConstructorRootOnly(loc); // observe (surprisingly)
 
     r
   }
@@ -87,6 +87,7 @@ module IndirectionTableImpl {
     linear garbageQueue: lOption<GarbageQueue>,
     refUpperBound: uint64,
     findLoclessIterator: Option<LinearMutableMap.SimpleIterator>)
+  class It
   {
 
     // method DebugAccumulate()
@@ -101,66 +102,66 @@ module IndirectionTableImpl {
     //   acc := DebugAccumulator.AccPut(acc, "garbageQueue", a);
     // }
 
-    protected predicate Inv()
+    static protected predicate Inv(me: indirectionTable)
     {
-      && LinearMutableMap.Inv(this.t)
-      && (this.garbageQueue.lSome? ==> USeq.Inv(this.garbageQueue.value))
+      && LinearMutableMap.Inv(me.t)
+      && (me.garbageQueue.lSome? ==> USeq.Inv(me.garbageQueue.value))
 
-      && var predCounts := IndirectionTableModel.PredCounts(this.t);
-      && var graph := IndirectionTableModel.Graph(this.t);
-      && var locs := IndirectionTableModel.Locs(this.t);
+      && var predCounts := IndirectionTableModel.PredCounts(me.t);
+      && var graph := IndirectionTableModel.Graph(me.t);
+      && var locs := IndirectionTableModel.Locs(me.t);
       && IndirectionTableModel.ValidPredCounts(predCounts, graph)
       && BC.GraphClosed(graph)
       && (forall ref | ref in graph :: |graph[ref]| <= MaxNumChildren())
-      && (this.garbageQueue.lSome? ==> (
-        && (forall ref | ref in this.t.contents && this.t.contents[ref].predCount == 0 :: ref in USeq.I(this.garbageQueue.value))
-        && (forall ref | ref in USeq.I(this.garbageQueue.value) :: ref in this.t.contents && this.t.contents[ref].predCount == 0)
+      && (me.garbageQueue.lSome? ==> (
+        && (forall ref | ref in me.t.contents && me.t.contents[ref].predCount == 0 :: ref in USeq.I(me.garbageQueue.value))
+        && (forall ref | ref in USeq.I(me.garbageQueue.value) :: ref in me.t.contents && me.t.contents[ref].predCount == 0)
       ))
-      && BT.G.Root() in this.t.contents
-      && this.t.count as int <= IndirectionTableModel.MaxSize()
-      && (forall ref | ref in graph :: ref <= this.refUpperBound)
-      && (this.findLoclessIterator.Some? ==>
-        && LinearMutableMap.WFSimpleIter(this.t, this.findLoclessIterator.value)
-        && (forall r | r in this.findLoclessIterator.value.s ::
+      && BT.G.Root() in me.t.contents
+      && me.t.count as int <= IndirectionTableModel.MaxSize()
+      && (forall ref | ref in graph :: ref <= me.refUpperBound)
+      && (me.findLoclessIterator.Some? ==>
+        && LinearMutableMap.WFSimpleIter(me.t, me.findLoclessIterator.value)
+        && (forall r | r in me.findLoclessIterator.value.s ::
             r in locs)
       )
     }
 
-    protected function I() : (res:IndirectionTableModel.IndirectionTable)
-    requires this.Inv()
+    static protected function I(me: indirectionTable) : (res:IndirectionTableModel.IndirectionTable)
+    requires Inv(me)
     ensures IndirectionTableModel.Inv(res)
     {
-      var res := IndirectionTableModel.FromHashMap(this.t, MapOption(this.garbageQueue.Option(), x => USeq.I(x)), this.refUpperBound, this.findLoclessIterator);
+      var res := IndirectionTableModel.FromHashMap(me.t, MapOption(me.garbageQueue.Option(), x => USeq.I(x)), me.refUpperBound, me.findLoclessIterator);
       IndirectionTableModel.reveal_Inv(res);
       res
     }
 
     // constructor RootOnly(loc: Location)
-    // ensures Inv()
+    // ensures Inv(me)
     // ensures fresh(Repr)
-    // ensures I() == IndirectionTableModel.ConstructorRootOnly(loc)
+    // ensures I(me) == IndirectionTableModel.ConstructorRootOnly(loc)
     // {
-    //   this.t := new LinearMutableMap.LinearHashMap(128);
-    //   this.findLoclessIterator := None;
+    //   me.t := new LinearMutableMap.LinearHashMap(128);
+    //   me.findLoclessIterator := None;
     //   new;
-    //   this.t.Insert(BT.G.Root(), IndirectionTableModel.Entry(Some(loc), [], 1));
-    //   this.garbageQueue := null;
-    //   this.refUpperBound := BT.G.Root();
-    //   Repr := {this} + this.t.Repr;
+    //   me.t.Insert(BT.G.Root(), IndirectionTableModel.Entry(Some(loc), [], 1));
+    //   me.garbageQueue := null;
+    //   me.refUpperBound := BT.G.Root();
+    //   Repr := {this} + me.t.Repr;
     //   IndirectionTableModel.reveal_ConstructorRootOnly();
     // }
 
     // constructor(t: HashMap)
-    // ensures this.t == t
-    // ensures this.garbageQueue == null
+    // ensures me.t == t
+    // ensures me.garbageQueue == null
     // {
-    //   this.t := t;
-    //   this.garbageQueue := null;
+    //   me.t := t;
+    //   me.garbageQueue := null;
     // }
 
-    linear method Destructor()
+    static method Destructor(linear me: indirectionTable)
     {
-      linear var indirectionTable(t, garbageQueue, refUpperBound, findLoclessIterator) := this;
+      linear var indirectionTable(t, garbageQueue, refUpperBound, findLoclessIterator) := me;
       LinearMutableMap.Destructor(t);
       linear match garbageQueue {
         case lNone => {}
@@ -168,45 +169,45 @@ module IndirectionTableImpl {
       }
     }
 
-    shared method Clone()
+    static method Clone(shared me: indirectionTable)
     returns (linear table : indirectionTable)
-    requires Inv()
-    ensures table.Inv()
-    ensures table.I() == IndirectionTableModel.clone(this.I())
+    requires Inv(me)
+    ensures Inv(table)
+    ensures I(table) == IndirectionTableModel.clone(I(me))
     {
       IndirectionTableModel.reveal_clone();
-      shared var indirectionTable(t, garbageQueue, refUpperBound, findLoclessIterator) := this;
+      shared var indirectionTable(t, garbageQueue, refUpperBound, findLoclessIterator) := me;
       linear var t' := LinearMutableMap.Clone(t);
       table := indirectionTable(t', lNone, refUpperBound, None);
     }
 
-    shared function method GetEntry(ref: BT.G.Reference) : (e : Option<IndirectionTableModel.Entry>)
-    requires Inv()
-    ensures e == IndirectionTableModel.GetEntry(I(), ref)
+    static function method GetEntry(shared me: indirectionTable, ref: BT.G.Reference) : (e : Option<IndirectionTableModel.Entry>)
+    requires Inv(me)
+    ensures e == IndirectionTableModel.GetEntry(I(me), ref)
     {
       IndirectionTableModel.reveal_GetEntry();
-      LinearMutableMap.Get(this.t, ref)
+      LinearMutableMap.Get(me.t, ref)
     }
 
-    shared function method HasEmptyLoc(ref: BT.G.Reference) : (b: bool)
-    requires Inv()
-    ensures b == IndirectionTableModel.HasEmptyLoc(I(), ref)
+    static function method HasEmptyLoc(shared me: indirectionTable, ref: BT.G.Reference) : (b: bool)
+    requires Inv(me)
+    ensures b == IndirectionTableModel.HasEmptyLoc(I(me), ref)
     {
-      var entry := LinearMutableMap.Get(this.t, ref);
+      var entry := LinearMutableMap.Get(me.t, ref);
       entry.Some? && entry.value.loc.None?
     }
 
-    linear method RemoveLoc(ref: BT.G.Reference)
+    static method RemoveLoc(linear me: indirectionTable, ref: BT.G.Reference)
     returns (linear self: indirectionTable, oldLoc: Option<Location>)
-    requires Inv()
-    requires IndirectionTableModel.TrackingGarbage(I())
-    requires ref in I().graph
-    ensures self.Inv()
-    ensures (self.I(), oldLoc) == IndirectionTableModel.RemoveLoc(I(), ref)
+    requires Inv(me)
+    requires IndirectionTableModel.TrackingGarbage(I(me))
+    requires ref in I(me).graph
+    ensures Inv(self)
+    ensures (I(self), oldLoc) == IndirectionTableModel.RemoveLoc(I(me), ref)
     {
       IndirectionTableModel.reveal_RemoveLoc();
 
-      linear var indirectionTable(t, garbageQueue, refUpperBound, findLoclessIterator) := this;
+      linear var indirectionTable(t, garbageQueue, refUpperBound, findLoclessIterator) := me;
       var it := LinearMutableMap.FindSimpleIter(t, ref);
       var oldEntry := LinearMutableMap.SimpleIterOutput(t, it);
       var predCount := oldEntry.value.predCount;
@@ -216,20 +217,20 @@ module IndirectionTableImpl {
 
       oldLoc := oldEntry.value.loc;
 
-      ghost var _ := IndirectionTableModel.RemoveLoc(old(I()), ref);
+      ghost var _ := IndirectionTableModel.RemoveLoc(old(I(me)), ref);
       self := indirectionTable(t, garbageQueue, refUpperBound, findLoclessIterator);
-      assert (self.I(), oldLoc) == IndirectionTableModel.RemoveLoc(I(), ref);
+      assert (I(self), oldLoc) == IndirectionTableModel.RemoveLoc(I(me), ref);
     }
 
-    linear method AddLocIfPresent(ref: BT.G.Reference, loc: Location)
+    static method AddLocIfPresent(linear me: indirectionTable, ref: BT.G.Reference, loc: Location)
     returns (linear self: indirectionTable, added: bool)
-    requires Inv()
-    ensures self.Inv()
-    ensures (self.I(), added) == IndirectionTableModel.AddLocIfPresent(I(), ref, loc)
+    requires Inv(me)
+    ensures Inv(self)
+    ensures (I(self), added) == IndirectionTableModel.AddLocIfPresent(I(me), ref, loc)
     {
       IndirectionTableModel.reveal_AddLocIfPresent();
 
-      linear var indirectionTable(t, garbageQueue, refUpperBound, findLoclessIterator) := this;
+      linear var indirectionTable(t, garbageQueue, refUpperBound, findLoclessIterator) := me;
       var it := LinearMutableMap.FindSimpleIter(t, ref);
       var oldEntry := LinearMutableMap.SimpleIterOutput(t, it);
       added := oldEntry.Next? && oldEntry.value.loc.None?;
@@ -237,33 +238,33 @@ module IndirectionTableImpl {
       if added {
         ghost var ghosty := true;
         if ghosty {
-          if I().findLoclessIterator.Some? {
-            LinearMutableMap.UpdatePreservesSimpleIter(I().t, it, IndirectionTableModel.Entry(Some(loc), oldEntry.value.succs, oldEntry.value.predCount), I().findLoclessIterator.value);
+          if I(me).findLoclessIterator.Some? {
+            LinearMutableMap.UpdatePreservesSimpleIter(I(me).t, it, IndirectionTableModel.Entry(Some(loc), oldEntry.value.succs, oldEntry.value.predCount), I(me).findLoclessIterator.value);
           }
         }
 
         t := LinearMutableMap.UpdateByIter(t, it, IndirectionTableModel.Entry(Some(loc), oldEntry.value.succs, oldEntry.value.predCount));
       }
 
-      ghost var _ := IndirectionTableModel.AddLocIfPresent(I(), ref, loc);
+      ghost var _ := IndirectionTableModel.AddLocIfPresent(I(me), ref, loc);
       self := indirectionTable(t, garbageQueue, refUpperBound, findLoclessIterator);
-      assert (self.I(), added) == IndirectionTableModel.AddLocIfPresent(I(), ref, loc);
+      assert (I(self), added) == IndirectionTableModel.AddLocIfPresent(I(me), ref, loc);
     }
 
-    linear method RemoveRef(ref: BT.G.Reference)
+    static method RemoveRef(linear me: indirectionTable, ref: BT.G.Reference)
     returns (linear self: indirectionTable, oldLoc : Option<Location>)
-    requires Inv()
-    requires IndirectionTableModel.TrackingGarbage(I())
-    requires IndirectionTableModel.deallocable(I(), ref)
-    ensures self.Inv()
-    ensures (self.I(), oldLoc) == IndirectionTableModel.RemoveRef(I(), ref)
+    requires Inv(me)
+    requires IndirectionTableModel.TrackingGarbage(I(me))
+    requires IndirectionTableModel.deallocable(I(me), ref)
+    ensures Inv(self)
+    ensures (I(self), oldLoc) == IndirectionTableModel.RemoveRef(I(me), ref)
     {
       IndirectionTableModel.reveal_RemoveRef();
 
-      IndirectionTableModel.lemma_count_eq_graph_size(I().t);
-      IndirectionTableModel.LemmaRemoveRefStuff(I(), ref);
+      IndirectionTableModel.lemma_count_eq_graph_size(I(me).t);
+      IndirectionTableModel.LemmaRemoveRefStuff(I(me), ref);
 
-      linear var indirectionTable(t, lSome(garbageQueue), refUpperBound, findLoclessIterator) := this;
+      linear var indirectionTable(t, lSome(garbageQueue), refUpperBound, findLoclessIterator) := me;
       linear var RemoveResult(t', oldEntry) := LinearMutableMap.RemoveAndGet(t, ref);
       t := t';
 
@@ -277,7 +278,7 @@ module IndirectionTableImpl {
       oldLoc := if oldEntry.Some? then oldEntry.value.loc else None;
       findLoclessIterator := None;
 
-      ghost var _ := IndirectionTableModel.RemoveRef(I(), ref);
+      ghost var _ := IndirectionTableModel.RemoveRef(I(me), ref);
       self := indirectionTable(t, lSome(garbageQueue), refUpperBound, findLoclessIterator);
     }
 
@@ -369,22 +370,22 @@ module IndirectionTableImpl {
       }
     }
 
-    linear method UpdateAndRemoveLoc(ref: BT.G.Reference, succs: seq<BT.G.Reference>)
+    static method UpdateAndRemoveLoc(linear me: indirectionTable, ref: BT.G.Reference, succs: seq<BT.G.Reference>)
     returns (linear self: indirectionTable, oldLoc : Option<Location>)
-    requires Inv()
-    requires IndirectionTableModel.TrackingGarbage(I())
+    requires Inv(me)
+    requires IndirectionTableModel.TrackingGarbage(I(me))
     requires |succs| <= MaxNumChildren()
-    requires |I().graph| < IndirectionTableModel.MaxSize()
-    requires IndirectionTableModel.SuccsValid(succs, I().graph)
-    ensures self.Inv()
-    ensures (self.I(), oldLoc)  == IndirectionTableModel.UpdateAndRemoveLoc(I(), ref, succs)
+    requires |I(me).graph| < IndirectionTableModel.MaxSize()
+    requires IndirectionTableModel.SuccsValid(succs, I(me).graph)
+    ensures Inv(self)
+    ensures (I(self), oldLoc)  == IndirectionTableModel.UpdateAndRemoveLoc(I(me), ref, succs)
     {
       IndirectionTableModel.reveal_UpdateAndRemoveLoc();
 
-      IndirectionTableModel.lemma_count_eq_graph_size(I().t);
-      IndirectionTableModel.LemmaUpdateAndRemoveLocStuff(I(), ref, succs);
+      IndirectionTableModel.lemma_count_eq_graph_size(I(me).t);
+      IndirectionTableModel.LemmaUpdateAndRemoveLocStuff(I(me), ref, succs);
 
-      linear var indirectionTable(t, lSome(garbageQueue), refUpperBound, findLoclessIterator) := this;
+      linear var indirectionTable(t, lSome(garbageQueue), refUpperBound, findLoclessIterator) := me;
       var oldEntry := LinearMutableMap.Get(t, ref);
       var predCount := if oldEntry.Some? then oldEntry.value.predCount else 0;
       if oldEntry.None? {
@@ -392,14 +393,14 @@ module IndirectionTableImpl {
       }
       t := LinearMutableMap.Insert(t, ref, IndirectionTableModel.Entry(None, succs, predCount));
 
-      IndirectionTableModel.lemma_count_eq_graph_size(this.t);
+      IndirectionTableModel.lemma_count_eq_graph_size(me.t);
 
       t, garbageQueue := UpdatePredCounts(t, garbageQueue, ref, succs,
           if oldEntry.Some? then oldEntry.value.succs else []);
 
-      IndirectionTableModel.lemma_count_eq_graph_size(this.t);
+      IndirectionTableModel.lemma_count_eq_graph_size(me.t);
 
-      //IndirectionTableModel.LemmaValidPredCountsOfValidPredCountsIntermediate(IndirectionTableModel.PredCounts(this.t), IndirectionTableModel.Graph(this.t), succs, if oldEntry.Some? then oldEntry.value.succs else []);
+      //IndirectionTableModel.LemmaValidPredCountsOfValidPredCountsIntermediate(IndirectionTableModel.PredCounts(me.t), IndirectionTableModel.Graph(me.t), succs, if oldEntry.Some? then oldEntry.value.succs else []);
 
       if ref > refUpperBound {
         refUpperBound := ref;
@@ -408,7 +409,7 @@ module IndirectionTableImpl {
       oldLoc := if oldEntry.Some? && oldEntry.value.loc.Some? then oldEntry.value.loc else None;
       findLoclessIterator := None;
 
-      ghost var _ := IndirectionTableModel.UpdateAndRemoveLoc(I(), ref, succs);
+      ghost var _ := IndirectionTableModel.UpdateAndRemoveLoc(I(me), ref, succs);
       self := indirectionTable(t, lSome(garbageQueue), refUpperBound, findLoclessIterator);
     }
 
@@ -620,9 +621,9 @@ module IndirectionTableImpl {
     static method ValToIndirectionTable(v: V)
     returns (linear s : lOption<indirectionTable>)
     requires IndirectionTableModel.valToIndirectionTable.requires(v)
-    ensures s.lSome? ==> s.value.Inv()
+    ensures s.lSome? ==> Inv(s.value)
     ensures s.lNone? ==> IndirectionTableModel.valToIndirectionTable(v).None?
-    ensures s.lSome? ==> IndirectionTableModel.valToIndirectionTable(v) == Some(s.value.I())
+    ensures s.lSome? ==> IndirectionTableModel.valToIndirectionTable(v) == Some(I(s.value))
     {
       if |v.a| as uint64 <= IndirectionTableModel.MaxSizeUint64() {
         linear var res := ValToHashMap(v.a);
@@ -664,7 +665,7 @@ module IndirectionTableImpl {
       8 + IndirectionTableModel.MaxSize() * (8 + 8 + 8 + (8 + MaxNumChildren() * 8))
     }
 
-    lemma lemma_SeqSum_prefix_array(a: array<V>, i: int)
+    static lemma lemma_SeqSum_prefix_array(a: array<V>, i: int)
     requires 0 < i <= a.Length
     ensures SeqSum(a[..i-1]) + SizeOfV(a[i-1]) == SeqSum(a[..i])
     {
@@ -672,14 +673,14 @@ module IndirectionTableImpl {
       assert a[..i-1] + [a[i-1]] == a[..i];
     }
 
-    lemma {:fuel SizeOfV,5} lemma_tuple_size(a: uint64, b: uint64, c: uint64, succs: seq<BT.G.Reference>)
+    static lemma {:fuel SizeOfV,5} lemma_tuple_size(a: uint64, b: uint64, c: uint64, succs: seq<BT.G.Reference>)
     requires|succs| <= MaxNumChildren()
     ensures SizeOfV(VTuple([VUint64(a), VUint64(b), VUint64(c), VUint64Array(succs)]))
          == (8 + 8 + 8 + (8 + |succs| * 8))
     {
     }
 
-    lemma lemma_SeqSum_empty()
+    static lemma lemma_SeqSum_empty()
     ensures SeqSum([]) == 0;
     {
       reveal_SeqSum();
@@ -881,8 +882,8 @@ module IndirectionTableImpl {
 
     // method marshallIndirectionTableContents(data: array<byte>, start: uint64)
     // returns (end: uint64)
-    // requires Inv()
-    // requires BC.WFCompleteIndirectionTable(IndirectionTableModel.I(I()))
+    // requires Inv(me)
+    // requires BC.WFCompleteIndirectionTable(IndirectionTableModel.I(I(me)))
 
     // requires 0 <= start as int <= data.Length
     // requires data.Length < 0x1_0000_0000_0000_0000
@@ -897,7 +898,7 @@ module IndirectionTableImpl {
     //          Marshalling.IndirectionTableRowGrammar(),
     //          t.Count
     //        )
-    //      ) == IndirectionTableModel.I(I())
+    //      ) == IndirectionTableModel.I(I(me))
     // {
     //   var idx := start;
     //   var it := t.IterStart();
@@ -908,8 +909,8 @@ module IndirectionTableImpl {
 
     // method marshallIndirectionTable(data: array<byte>, start_idx: uint64)
     // returns (end: uint64)
-    // requires Inv()
-    // requires BC.WFCompleteIndirectionTable(IndirectionTableModel.I(I()))
+    // requires Inv(me)
+    // requires BC.WFCompleteIndirectionTable(IndirectionTableModel.I(I(me)))
     // modifies data
     // {
     //   var idx := start_idx;
@@ -955,33 +956,33 @@ module IndirectionTableImpl {
     // but it's kind of annoying. However, I think that it won't
     // be a big deal as long as most syncs are journaling syncs?
     // So I've moved back to this one which is slower but cleaner.
-    shared method indirectionTableToVal()
+    static method indirectionTableToVal(shared me: indirectionTable)
     returns (v : V, size: uint64)
-    requires Inv()
-    requires BC.WFCompleteIndirectionTable(IndirectionTableModel.I(I()))
+    requires Inv(me)
+    requires BC.WFCompleteIndirectionTable(IndirectionTableModel.I(I(me)))
     ensures ValInGrammar(v, IndirectionTableModel.IndirectionTableGrammar())
     ensures ValidVal(v)
     ensures IndirectionTableModel.valToIndirectionTable(v).Some?
     ensures
           IndirectionTableModel.I(IndirectionTableModel.valToIndirectionTable(v).value)
-       == IndirectionTableModel.I(I())
+       == IndirectionTableModel.I(I(me))
     ensures SizeOfV(v) <= MaxIndirectionTableByteSize()
     ensures SizeOfV(v) == size as int
     {
-      assert t.count <= IndirectionTableModel.MaxSizeUint64();
+      assert me.t.count <= IndirectionTableModel.MaxSizeUint64();
       lemma_SeqSum_empty();
-      var count := t.count as uint64;
+      var count := me.t.count as uint64;
       var a: array<V> := new V[count];
-      var it := LinearMutableMap.IterStart(t);
+      var it := LinearMutableMap.IterStart(me.t);
       var i: uint64 := 0;
       size := 0;
 
       ghost var partial := map[];
       while it.next.Next?
-      invariant Inv()
-      invariant BC.WFCompleteIndirectionTable(IndirectionTableModel.I(I()))
+      invariant Inv(me)
+      invariant BC.WFCompleteIndirectionTable(IndirectionTableModel.I(I(me)))
       invariant 0 <= i as int <= a.Length
-      invariant LinearMutableMap.WFIter(t, it);
+      invariant LinearMutableMap.WFIter(me.t, it);
       invariant forall j | 0 <= j < i :: ValidVal(a[j])
       invariant forall j | 0 <= j < i :: ValInGrammar(a[j], GTuple([GUint64, GUint64, GUint64, GUint64Array]))
       // NOALIAS/CONST table doesn't need to be mutable, if we could say so we wouldn't need this
@@ -989,19 +990,19 @@ module IndirectionTableImpl {
       invariant IndirectionTableModel.valToHashMap(a[..i]).value.contents == partial
       invariant |partial.Keys| == i as nat
       invariant partial.Keys == it.s
-      invariant partial.Keys <= t.contents.Keys
-      invariant forall r | r in partial :: r in t.contents
-          && partial[r].loc == t.contents[r].loc
-          && partial[r].succs == t.contents[r].succs
+      invariant partial.Keys <= me.t.contents.Keys
+      invariant forall r | r in partial :: r in me.t.contents
+          && partial[r].loc == me.t.contents[r].loc
+          && partial[r].succs == me.t.contents[r].succs
       // NOALIAS/CONST t doesn't need to be mutable, if we could say so we wouldn't need this
-      invariant t.contents == old(t.contents)
+      invariant me.t.contents == old(me.t.contents)
       invariant size as int <=
           |it.s| * (8 + 8 + 8 + (8 + MaxNumChildren() * 8))
       invariant SeqSum(a[..i]) == size as int;
       decreases it.decreaser
       {
         var (ref, locOptGraph: IndirectionTableModel.Entry) := (it.next.key, it.next.value);
-        assert ref in I().locs;
+        assert ref in I(me).locs;
         // NOTE: deconstructing in two steps to work around c# translation bug
         var locOpt := locOptGraph.loc;
         var succs := locOptGraph.succs;
@@ -1011,11 +1012,11 @@ module IndirectionTableImpl {
 
         assert |succs| <= MaxNumChildren();
 
-        //assert I().locs[ref] == loc;
-        //assert I().graph[ref] == succs;
+        //assert I(me).locs[ref] == loc;
+        //assert I(me).graph[ref] == succs;
 
-        //assert IndirectionTableModel.I(I()).locs[ref] == loc;
-        //assert IndirectionTableModel.I(I()).graph[ref] == succs;
+        //assert IndirectionTableModel.I(I(me)).locs[ref] == loc;
+        //assert IndirectionTableModel.I(I(me)).graph[ref] == succs;
 
         assert ValidNodeLocation(loc);
         /*ghost var t0 := IndirectionTableModel.valToHashMap(a[..i]);
@@ -1023,12 +1024,12 @@ module IndirectionTableImpl {
         assert loc.addr != 0;
         assert LBAType.ValidLocation(loc);*/
 
-        LinearMutableMap.LemmaIterIndexLtCount(t, it);
+        LinearMutableMap.LemmaIterIndexLtCount(me.t, it);
 
         assert |succs| < 0x1_0000_0000_0000_0000;
         assert ValidVal(VTuple([VUint64(ref), VUint64(loc.addr), VUint64(loc.len), childrenVal]));
 
-        assert |LinearMutableMap.IterInc(t, it).s| == |it.s| + 1;
+        assert |LinearMutableMap.IterInc(me.t, it).s| == |it.s| + 1;
 
         var vi := VTuple([VUint64(ref), VUint64(loc.addr), VUint64(loc.len), childrenVal]);
 
@@ -1038,7 +1039,7 @@ module IndirectionTableImpl {
         partial := partial[ref := IndirectionTableModel.Entry(locOpt, succs, 0)];
         a[i] := vi;
         i := i + 1;
-        it := LinearMutableMap.IterInc(t, it);
+        it := LinearMutableMap.IterInc(me.t, it);
         // ==============
 
         assert a[..i-1] == DropLast(a[..i]); // observe
@@ -1059,8 +1060,8 @@ module IndirectionTableImpl {
         size := size + 32 + 8 * |succs| as uint64;
       }
 
-      /* (doc) assert |partial.Keys| == |t.contents.Keys|; */
-      SetInclusionAndEqualCardinalityImpliesSetEquality(partial.Keys, t.contents.Keys);
+      /* (doc) assert |partial.Keys| == |me.t.contents.Keys|; */
+      SetInclusionAndEqualCardinalityImpliesSetEquality(partial.Keys, me.t.contents.Keys);
 
       assert a[..i] == a[..]; // observe
       v := VArray(a[..]);
@@ -1107,38 +1108,38 @@ module IndirectionTableImpl {
       BitmapInitUpToIterate(bm, 0, upTo);
     }
 
-    shared method InitLocBitmap()
+    static method InitLocBitmap(shared me: indirectionTable)
     returns (success: bool, bm: BitmapImpl.Bitmap)
-    requires Inv()
-    requires BC.WFCompleteIndirectionTable(IndirectionTableModel.I(I()))
+    requires Inv(me)
+    requires BC.WFCompleteIndirectionTable(IndirectionTableModel.I(I(me)))
     ensures bm.Inv()
-    ensures (success, bm.I()) == IndirectionTableModel.InitLocBitmap(old(I()))
+    ensures (success, bm.I()) == IndirectionTableModel.InitLocBitmap(old(I(me)))
     ensures fresh(bm.Repr)
     {
       IndirectionTableModel.reveal_InitLocBitmap();
 
       bm := new BitmapImpl.Bitmap(NumBlocksUint64());
       BitmapInitUpTo(bm, MinNodeBlockIndexUint64());
-      var it := LinearMutableMap.IterStart(t);
+      var it := LinearMutableMap.IterStart(me.t);
       while it.next.Next?
-      invariant t.Inv()
-      invariant BC.WFCompleteIndirectionTable(IndirectionTableModel.I(I()))
+      invariant me.t.Inv()
+      invariant BC.WFCompleteIndirectionTable(IndirectionTableModel.I(I(me)))
       invariant bm.Inv()
-      invariant LinearMutableMap.WFIter(t, it)
+      invariant LinearMutableMap.WFIter(me.t, it)
       invariant BitmapModel.Len(bm.I()) == NumBlocks()
-      invariant IndirectionTableModel.InitLocBitmapIterate(I(), it, bm.I())
-             == IndirectionTableModel.InitLocBitmap(I())
+      invariant IndirectionTableModel.InitLocBitmapIterate(I(me), it, bm.I())
+             == IndirectionTableModel.InitLocBitmap(I(me))
       invariant fresh(bm.Repr)
       decreases it.decreaser
       {
-        assert it.next.key in IndirectionTableModel.I(I()).locs;
+        assert it.next.key in IndirectionTableModel.I(I(me)).locs;
 
         var loc: uint64 := it.next.value.loc.value.addr;
         var locIndex: uint64 := loc / NodeBlockSizeUint64();
         if locIndex < NumBlocksUint64() {
           var isSet := bm.GetIsSet(locIndex);
           if !isSet {
-            it := LinearMutableMap.IterInc(t, it);
+            it := LinearMutableMap.IterInc(me.t, it);
             bm.Set(locIndex);
           } else {
             success := false;
@@ -1155,31 +1156,31 @@ module IndirectionTableImpl {
     
     ///// Dealloc stuff
 
-    shared function method FindDeallocable() : (ref: Option<BT.G.Reference>)
-    requires Inv()
-    requires IndirectionTableModel.TrackingGarbage(I())
-    ensures ref == IndirectionTableModel.FindDeallocable(I())
+    static function method FindDeallocable(shared me: indirectionTable) : (ref: Option<BT.G.Reference>)
+    requires Inv(me)
+    requires IndirectionTableModel.TrackingGarbage(I(me))
+    ensures ref == IndirectionTableModel.FindDeallocable(I(me))
     {
       IndirectionTableModel.reveal_FindDeallocable();
-      USeq.FirstOpt(garbageQueue.value)
+      USeq.FirstOpt(me.garbageQueue.value)
     }
 
-    shared function method GetSize() : (size: uint64)
-    requires Inv()
-    ensures size as int == |I().graph|
+    static function method GetSize(shared me: indirectionTable) : (size: uint64)
+    requires Inv(me)
+    ensures size as int == |I(me).graph|
     {
-      IndirectionTableModel.lemma_count_eq_graph_size(I().t);
-      this.t.count
+      IndirectionTableModel.lemma_count_eq_graph_size(I(me).t);
+      me.t.count
     }
 
-    linear method FindRefWithNoLoc() returns (linear self: indirectionTable, ref: Option<BT.G.Reference>)
-    requires Inv()
-    ensures self.Inv()
-    ensures (self.I(), ref) == IndirectionTableModel.FindRefWithNoLoc(I())
+    static method FindRefWithNoLoc(linear me: indirectionTable) returns (linear self: indirectionTable, ref: Option<BT.G.Reference>)
+    requires Inv(me)
+    ensures Inv(self)
+    ensures (I(self), ref) == IndirectionTableModel.FindRefWithNoLoc(I(me))
     {
       IndirectionTableModel.reveal_FindRefWithNoLoc();
 
-      linear var indirectionTable(t, garbageQueue, refUpperBound, findLoclessIterator) := this;
+      linear var indirectionTable(t, garbageQueue, refUpperBound, findLoclessIterator) := me;
       var it;
       if findLoclessIterator.Some? {
         it := findLoclessIterator.value;
@@ -1188,12 +1189,12 @@ module IndirectionTableImpl {
       }
 
       while true
-      invariant Inv()
+      invariant Inv(me)
       invariant LinearMutableMap.WFSimpleIter(t, it)
-      invariant forall r | r in it.s :: r in I().locs
-      invariant IndirectionTableModel.FindRefWithNoLoc(I())
+      invariant forall r | r in it.s :: r in I(me).locs
+      invariant IndirectionTableModel.FindRefWithNoLoc(I(me))
           == IndirectionTableModel.FindRefWithNoLocIterate(
-              indirectionTable(t, garbageQueue, refUpperBound, findLoclessIterator).I(), it)
+              I(indirectionTable(t, garbageQueue, refUpperBound, findLoclessIterator)), it)
       decreases it.decreaser
       {
         var next := LinearMutableMap.SimpleIterOutput(t, it);
@@ -1214,12 +1215,12 @@ module IndirectionTableImpl {
       self := indirectionTable(t, garbageQueue, refUpperBound, findLoclessIterator);
     }
 
-    shared function method GetRefUpperBound() : (r: uint64)
-    requires Inv()
-    ensures r == IndirectionTableModel.getRefUpperBound(this.I())
+    static function method GetRefUpperBound(shared me: indirectionTable) : (r: uint64)
+    requires Inv(me)
+    ensures r == IndirectionTableModel.getRefUpperBound(I(me))
     {
       IndirectionTableModel.reveal_getRefUpperBound();
-      this.refUpperBound
+      me.refUpperBound
     }
   }
 
@@ -1255,7 +1256,7 @@ module IndirectionTableImpl {
       && Repr == {this} + box.Repr
       && box.Inv()
       && box.Has()
-      && Read().Inv()
+      && It.Inv(Read())
     }
 
     protected function I() : IndirectionTableModel.IndirectionTable
@@ -1263,7 +1264,7 @@ module IndirectionTableImpl {
       requires Inv()
       ensures IndirectionTableModel.Inv(I())
     {
-      Read().I()
+      It.I(Read())
     }
 
     constructor Box(box: BoxedLinear<indirectionTable>)
@@ -1306,7 +1307,7 @@ module IndirectionTableImpl {
       modifies Repr
     {
       linear var x := box.Take();
-      x.Destructor();
+      It.Destructor(x);
     }
 
     method Clone() returns (table: IndirectionTable)
@@ -1318,7 +1319,7 @@ module IndirectionTableImpl {
       ensures table.I() == IndirectionTableModel.clone(old(I()))
     {
       linear var x := box.Take();
-      linear var clone := x.Clone();
+      linear var clone := It.Clone(x);
       box.Give(x);
       var boxed := new BoxedLinear(clone);
       table := new IndirectionTable.Box(boxed);
@@ -1329,7 +1330,7 @@ module IndirectionTableImpl {
       reads Repr
       ensures e == IndirectionTableModel.GetEntry(I(), ref)
     {
-      box.Borrow().GetEntry(ref)
+      It.GetEntry(box.Borrow(), ref)
     }
 
     function method HasEmptyLoc(ref: BT.G.Reference) : (b: bool)
@@ -1337,7 +1338,7 @@ module IndirectionTableImpl {
       reads Repr
       ensures b == IndirectionTableModel.HasEmptyLoc(I(), ref)
     {
-      box.Borrow().HasEmptyLoc(ref)
+      It.HasEmptyLoc(box.Borrow(), ref)
     }
 
     method RemoveLoc(ref: BT.G.Reference) returns (oldLoc: Option<Location>)
@@ -1350,7 +1351,7 @@ module IndirectionTableImpl {
       ensures (I(), oldLoc) == IndirectionTableModel.RemoveLoc(old(I()), ref)
     {
       linear var x := box.Take();
-      x, oldLoc := x.RemoveLoc(ref);
+      x, oldLoc := It.RemoveLoc(x, ref);
       box.Give(x);
     }
 
@@ -1362,7 +1363,7 @@ module IndirectionTableImpl {
       ensures (I(), added) == IndirectionTableModel.AddLocIfPresent(old(I()), ref, loc)
     {
       linear var x := box.Take();
-      x, added := x.AddLocIfPresent(ref, loc);
+      x, added := It.AddLocIfPresent(x, ref, loc);
       box.Give(x);
     }
 
@@ -1376,7 +1377,7 @@ module IndirectionTableImpl {
       ensures (I(), oldLoc) == IndirectionTableModel.RemoveRef(old(I()), ref)
     {
       linear var x := box.Take();
-      x, oldLoc := x.RemoveRef(ref);
+      x, oldLoc := It.RemoveRef(x, ref);
       box.Give(x);
     }
 
@@ -1392,7 +1393,7 @@ module IndirectionTableImpl {
       ensures (I(), oldLoc) == IndirectionTableModel.UpdateAndRemoveLoc(old(I()), ref, succs)
     {
       linear var x := box.Take();
-      x, oldLoc := x.UpdateAndRemoveLoc(ref, succs);
+      x, oldLoc := It.UpdateAndRemoveLoc(x, ref, succs);
       box.Give(x);
     }
 
@@ -1403,7 +1404,7 @@ module IndirectionTableImpl {
       ensures s == null ==> IndirectionTableModel.valToIndirectionTable(v).None?
       ensures s != null ==> IndirectionTableModel.valToIndirectionTable(v) == Some(s.I())
     {
-      linear var opt := indirectionTable.ValToIndirectionTable(v);
+      linear var opt := It.ValToIndirectionTable(v);
       linear match opt {
         case lNone => {s := null;}
         case lSome(it) => {
@@ -1424,11 +1425,11 @@ module IndirectionTableImpl {
       ensures
             IndirectionTableModel.I(IndirectionTableModel.valToIndirectionTable(v).value)
          == IndirectionTableModel.I(I())
-      ensures SizeOfV(v) <= indirectionTable.MaxIndirectionTableByteSize()
+      ensures SizeOfV(v) <= It.MaxIndirectionTableByteSize()
       ensures SizeOfV(v) == size as int
     {
       linear var x := box.Take();
-      v, size := x.indirectionTableToVal();
+      v, size := It.indirectionTableToVal(x);
       box.Give(x);
     }
 
@@ -1442,7 +1443,7 @@ module IndirectionTableImpl {
       ensures fresh(bm.Repr)
     {
       linear var x := box.Take();
-      success, bm := x.InitLocBitmap();
+      success, bm := It.InitLocBitmap(x);
       box.Give(x);
     }
     
@@ -1452,7 +1453,7 @@ module IndirectionTableImpl {
       reads Repr
       ensures ref == IndirectionTableModel.FindDeallocable(I())
     {
-      box.Borrow().FindDeallocable()
+      It.FindDeallocable(box.Borrow())
     }
 
     function method GetSize() : (size: uint64)
@@ -1460,7 +1461,7 @@ module IndirectionTableImpl {
       reads Repr
       ensures size as int == |I().graph|
     {
-      box.Borrow().GetSize()
+      It.GetSize(box.Borrow())
     }
 
     method FindRefWithNoLoc() returns (ref: Option<BT.G.Reference>)
@@ -1471,7 +1472,7 @@ module IndirectionTableImpl {
       ensures (I(), ref) == IndirectionTableModel.FindRefWithNoLoc(old(I()))
     {
       linear var x := box.Take();
-      x, ref := x.FindRefWithNoLoc();
+      x, ref := It.FindRefWithNoLoc(x);
       box.Give(x);
     }
 
@@ -1480,7 +1481,7 @@ module IndirectionTableImpl {
       reads Repr
       ensures r == IndirectionTableModel.getRefUpperBound(this.I())
     {
-      box.Borrow().GetRefUpperBound()
+      It.GetRefUpperBound(box.Borrow())
     }
   }
 }
